Added separate interface for tables. Finished hashtable impl with finite maps. Added iris table_inv. Added new version of test clients.

iterators/hashtable_model.v
@@ -1,9 +1,8 @@
-From iris.heap_lang Require Import lang notation proofmode.
-From iris.prelude Require Import list fin_maps.
+From stdpp Require Export list fin_maps.
 From iris.program_logic Require Import hoare.
+From iris.heap_lang Require Export lifting notation.
 From iris_programs.iterators Require Import util.
 
-  
 Class Hashable Σ `{heapG Σ} (Key : Type) `{EqDecision Key} (Hash : Key -> nat) :=
   { equalf : val;
     hashf : val;
@@ -64,55 +63,169 @@ Section model.
     rewrite /remove_val insert_proper ; [reflexivity..|by rewrite Heq | assumption].
   Qed.
 
-  Global Instance all_elements_proper : Proper (MEquiv ==> (≡ₚ)) all_elements.
+  Lemma table_ind :
+    forall (P : Map (list val) -> Prop),
+    Proper ( MEquiv ==> (↔)) P ->
+    P ∅ -> (∀ k x M, P M → P (insert_val M k x)) → ∀ M, P M.
   Proof.
-    assert ( ∀ (k : Key) (l : list val),
-               Proper (Permutation ==> Permutation)
-                      (λ acc, ((λ v, (k, v)) <$> l) ++ acc)) by solve_proper.
-    
-    assert (∀ (l1 l2 l3 : list (Key * val)),
-               l1 ++ l2 ++ l3 ≡ₚ l2 ++ l1 ++ l3).
-    { intros. do 2 rewrite app_assoc. f_equiv. apply Permutation_app_comm. }
-    
-    intros M1. unfold all_elements.
-    induction M1 as [|k x M1 Hlookup IH] using map_ind ; intros M2.
-    - induction M2 as [|k x M2 Hlookup IH] using map_ind.
+    intros P ? Hempty Hind M.
+    induction M as [|k l M Hlookup IHM] using map_ind. assumption.
+    induction l.
+    - rewrite (_:MEquiv (<[k:=[]]> M) M). assumption.
+      intros k'. unfold lookup_all.
+      destruct (decide (k = k')) as [<-|].
+      + by rewrite Hlookup lookup_insert. 
+      + by rewrite lookup_insert_ne.
+    - unfold insert_val in Hind.
+      rewrite -(insert_insert _ _ _ l).
+      rewrite {1}(_: l = lookup_all (<[k:=l]> M) k).
+      auto. by rewrite /lookup_all lookup_insert.
+  Qed.      
+
+  Lemma MEquiv_proper `(R : relation B) (f : Key -> list val -> B -> B) fM `{!Equivalence R} :
+    Proper ((=) ==> (=) ==> R ==> R) f -> 
+    (forall k l M, M !! k = None -> R (f k l (fM M)) (fM (<[k:=l]>M))) ->
+    (forall M k, R (f k [] (fM M)) (fM M))  ->
+    Proper (MEquiv ==> R) fM.
+  Proof.
+    intros ? Hinsert Hnil M1. induction M1 as [|k l M1 Hlookup IH]  using map_ind.
+    - intro M2. induction M2 as [|k l M2 Hlookup IH] using map_ind.
       + reflexivity.
-      + intro Heq.
-        rewrite (map_fold_insert Permutation) ; last assumption.
-        pose proof Heq as Heq_cpy.
-        unfold MEquiv, lookup_all in Heq_cpy. specialize (Heq_cpy k).
-        rewrite lookup_empty lookup_insert /= in Heq_cpy.
-        rewrite -Heq_cpy. apply IH.
-        rewrite Heq. intro k'. destruct (decide (k = k')) as [<- |].
-        by rewrite /lookup_all lookup_insert Hlookup.
-        by rewrite /lookup_all lookup_insert_ne.
-        done.
-    - intro Heq. case_eq (M2 !! k).
-      + intros l Hl.
-        rewrite -(insert_id _ _ _ Hl) -(insert_delete M2).
-        rewrite (map_fold_insert Permutation) ; last assumption.
-        rewrite (map_fold_insert Permutation) ; last apply lookup_delete.
-        rewrite IH. do 2 f_equiv. specialize (Heq k). rewrite /lookup_all Hl lookup_insert /= in Heq.
-        rewrite Heq. reflexivity.
+      + intros Heq.
+        assert (MEquiv ∅ M2).
+        { intro k'. rewrite /lookup_all. destruct (decide (k = k')) as [<-|].
+          - by rewrite Hlookup lookup_empty.
+          - specialize (Heq k'). by rewrite /lookup_all lookup_insert_ne in Heq.
+        }
+        specialize (Heq k). rewrite /lookup_all lookup_insert lookup_empty /= in Heq.
+        simplify_eq. rewrite -Hinsert ; last assumption. rewrite Hnil. auto.
+    - intros M2 Heq.
+      pose proof Heq as HeqCpy. specialize (HeqCpy k).
+      rewrite /lookup_all lookup_insert in HeqCpy.
+      rewrite -Hinsert ; last assumption.
+      case_eq (M2 !! k).
+      + intros l' Hl'. simpl.
+        rewrite Hl' /= in HeqCpy. simplify_eq.
+        rewrite -(insert_id _ _ _ Hl') -insert_delete.
+        rewrite -Hinsert ; last apply lookup_delete. f_equiv.
+        apply IH.
         intro k'. destruct (decide (k = k')) as [<- |].
-        by rewrite /lookup_all lookup_delete Hlookup.
-        rewrite /lookup_all lookup_delete_ne.
-        rewrite -(lookup_insert_ne M1 k k' x). apply Heq. all : done.
-      + intros HNone.
-        rewrite -(delete_notin _ _ HNone).
-        rewrite (map_fold_insert Permutation) ; last assumption.
-        rewrite IH. specialize (Heq k). rewrite /lookup_all HNone lookup_insert /= in Heq.
-        rewrite Heq /=. reflexivity.
+        * by rewrite /lookup_all lookup_delete Hlookup.
+        * rewrite /lookup_all lookup_delete_ne ; last assumption.
+          specialize (Heq k'). by rewrite /lookup_all lookup_insert_ne in Heq. 
+      + intro HNone. rewrite HNone /=in HeqCpy. simplify_eq.
+        rewrite Hnil. apply IH.
         intro k'. destruct (decide (k = k')) as [<- |].
-        by rewrite /lookup_all lookup_delete Hlookup.
-        rewrite /lookup_all lookup_delete_ne.
-        rewrite -(lookup_insert_ne M1 k k' x). apply Heq. all : done.
+        * by rewrite /lookup_all Hlookup HNone.
+        * specialize (Heq k'). by rewrite /lookup_all lookup_insert_ne in Heq.
   Qed.
   
+  Global Instance all_elements_proper : Proper (MEquiv ==> (≡ₚ)) all_elements.
+  Proof.
+    apply (MEquiv_proper _ (fun k l acc => ((fun v => (k, v)) <$> l) ++ acc)).
+    typeclasses eauto. solve_proper.
+    intros. unfold all_elements. erewrite (map_fold_insert Permutation). reflexivity. solve_proper.
+    intros. do 2 rewrite app_assoc. f_equiv. apply Permutation_app_comm.
+    assumption. reflexivity.
+  Qed.
+    
+  Inductive removal : Map (list val) -> list (val * val) -> Map (list val) -> Prop :=
+  | RemovalNil {M M'} : MEquiv M M' -> removal M [] M'
+  | RemovalCons {k k' x l M M' M''} :
+      as_key k = Some k' ->
+      head (lookup_all M k') = Some x ->
+      MEquiv M' (remove_val M k') ->
+      removal M' l M'' ->
+      removal M ((k, x) :: l) M''.
+
+  Global Instance removal_proper : Proper (MEquiv ==> (=) ==> MEquiv ==> (↔)) removal.
+  Proof.
+    intros M1 M2 HMeq seq? <- M1' M2' HMeq'.
+    assert (forall M1 M2 M1' M2', MEquiv M1 M2 -> MEquiv M1' M2' ->
+                                  removal M1 seq M1' -> removal M2 seq M2').
+    { clear dependent M1 M2 M1' M2'.
+      induction seq as [|? ? IH] ; intros M1 M2 M1' M2' HMeq HMeq' Hrem.
+      - inversion Hrem. constructor. congruence.
+      - inversion Hrem as [| ????? M']. simplify_eq. econstructor ; [done|by rewrite -HMeq..|].
+        by apply (IH M' _ M1').
+    }
+    split ; last symmetry in HMeq, HMeq' ; eauto.
+  Qed.       
+    
+  Lemma removal_app_1 M seq M' seq' M'':
+    removal M seq M' ->
+    removal M' seq' M'' ->
+    removal M (seq ++ seq') M''.
+  Proof.
+    intro HRem. induction HRem as [???Heq|] ; [by rewrite Heq | econstructor ; eauto].
+  Qed.
+  
+  Lemma removal_app_2 M M' seq seq' :
+    removal M (seq ++ seq') M' ->
+    exists M'', removal M seq M'' /\ removal M'' seq' M'. 
+  Proof.
+    revert M.
+    induction seq as [|[k x] seq IH].
+    - simpl. intros M ?. exists M. split. by constructor 1. assumption.
+    - simpl. intros M Hrem. inversion Hrem as [| ? k' ???????? Hrem']. simplify_eq.
+      specialize (IH (delete k' M) Hrem'). destruct IH as [M'' [Hseq Hseq']].
+      exists M''. split.
+      by econstructor. assumption.
+  Qed.
+
+  Definition permitted M seq := exists M', removal M seq M'.
+  Definition complete M seq := removal M seq ∅ .
+
+  Global Instance permitted_proper : Proper (MEquiv ==> (=) ==> (↔)) permitted.
+  Proof. solve_proper. Qed.
+        
+  Lemma complete_all_elements M seq:
+    complete M seq ->
+    exists seq', Forall2 (fun '(k, x) '(k', x') => x = x' /\ as_key k' = Some k) seq' seq /\
+                 seq' ≡ₚ all_elements M.
+  Proof.
+    pose proof all_elements_proper.
+    assert (forall (k : Key) (l : list val),
+               Proper (Permutation ==> Permutation) (fun acc => ((fun x => (k, x)) <$> l) ++ acc)).
+    { solve_proper. }
+    assert ( forall A (l1 l2 l3 : list A),
+               l1 ++ l2 ++ l3 ≡ₚ l2 ++ l1 ++ l3).
+    { intros. do 2 rewrite app_assoc. f_equiv. Search app. apply Permutation_app_comm. }
+    revert M. induction seq as [|[k x] seq IH].
+    - intros M HCom. exists [].
+      split ; first done. inversion HCom as [???HEq|].
+       by rewrite HEq /all_elements map_fold_empty.
+    - intros M HCom. inversion HCom as [| ??k'??????? HEq HRem].
+      specialize (IH _ HRem). destruct IH as [seq' [Hforall HPerm]].
+      exists ((k', x) :: seq'). split.
+      + by apply Forall2_cons.
+      +  rewrite HPerm HEq /all_elements /remove_val -insert_delete.
+         rewrite (map_fold_insert Permutation) ; [|done|apply lookup_delete].
+         rewrite app_comm_cons  -fmap_cons.
+         assert (Hlookup_all: x :: tail (lookup_all M k') = lookup_all M k').
+         { symmetry. by apply hd_error_tl_repr. }
+         assert (Hlookup : M !! k' = Some (x :: tail (lookup_all M k'))).
+         {
+           rewrite Hlookup_all /lookup_all.
+           rewrite {2}/lookup_all in Hlookup_all.
+           symmetry in Hlookup_all. apply from_option_inv_ne in Hlookup_all.
+           by destruct Hlookup_all as [? ->]. done.
+         }
+         rewrite Hlookup_all.
+         rewrite <-(map_fold_insert Permutation
+                                     (fun k l acc => ((fun x => (k, x)) <$> l) ++ acc) _
+                                     k' (lookup_all M k')) ; [|done..|apply lookup_delete].
+         rewrite insert_delete. rewrite insert_id. reflexivity. by rewrite Hlookup Hlookup_all.
+  Qed.        
+    
+  Global Instance complete_proper : Proper (MEquiv ==> (=) ==> (↔)) complete.
+  Proof. solve_proper. Qed.
+
+  
+      
 End model.
 
-Structure Table Σ Key Hash `{Hashable Σ Key Hash} Map `{FinMap Key Map} :=
+Structure Table Σ Key Hash `{Hashable Σ Key Hash} Map `{FinMap Key Map} : Type :=
   { table_create : val ;
     table_insert : val ;
     table_lookup : val ;
@@ -121,19 +234,12 @@ Structure Table Σ Key Hash `{Hashable Σ Key Hash} Map `{FinMap Key Map} :=
 
     table_state : Type ;
     table_in_state : Map (list val) -> table_state -> val -> iProp Σ ;
-    permitted : Map (list val) -> list (Key * val) -> Prop ;
-    complete : Map (list val) -> list (Key * val) -> Prop ;
-    is_cascade : val -> list (Key * val) -> table_state -> val -> Prop ;
+    is_cascade : Map (list val) -> val -> list (val * val) -> table_state -> val -> Prop ;
 
-    table_in_state_proper: Proper (MEquiv ==> (=) ==> (=) ==> (↔)) table_in_state ;
-    permitted_proper : Proper (MEquiv ==> (=) ==> (↔)) permitted ;
-    complete_proper : Proper (MEquiv ==> (=) ==> (↔)) complete ;
+    table_in_state_proper: Proper (MEquiv ==> (=) ==> (=) ==> (⊣⊢)) table_in_state ;
+    is_cascade_proper : Proper (MEquiv ==> (=) ==> (=) ==> (=) ==> (=) ==> (↔)) is_cascade ;
     
-    complete_all_elements M seq: complete M seq -> seq ≡ₚ all_elements M ;
-    complete_permitted M seq : complete M seq -> permitted M seq ;
-    permitted_prefix M seq seq': permitted M seq -> seq' `prefix_of` seq -> permitted M seq' ;
-    
-    table_create_spec n : n > 0 -> WP table_create #n {{t, ∃ state, table_in_state ∅ state t}}%I ;
+    table_create_spec (n : nat) : (n > 0)%nat -> WP table_create #n {{t, ∃ state, table_in_state ∅ state t}}%I ;
     
     table_insert_spec (t k x : val) M state k' :
       as_key k = Some k' ->
@@ -151,27 +257,44 @@ Structure Table Σ Key Hash `{Hashable Σ Key Hash} Map `{FinMap Key Map} :=
             table_in_state M state t }}} ;
 
     table_fold_spec M state I (f t a : val) :
-      (forall k k' x seq (a' : val),
-          as_key k = Some k' ->
-          permitted M (seq ++ [(k', x)]) ->
-          {{I seq a'}} f k x a' {{v,I (seq ++ [(k' ,x)]) v }}%I) ->
+      (forall k x seq (a' : val),
+          permitted M (seq ++ [(k, x)]) ->
+          {{I seq a'}} f k x a' {{v,I (seq ++ [(k ,x)]) v }}%I) ->
       {{{table_in_state M state t ∗ I [] a}}}
         table_fold f t a
         {{{v seq, RET v; ⌜complete M seq⌝ ∗ table_in_state M state t ∗ I seq v}}} ;
 
     is_cascade_spec M f seq state t:
-      is_cascade f seq state t ->
+      is_cascade M f seq state t ->
       {{{ table_in_state M state t }}}
         f #()
-        {{{v k k' x f' , RET v; table_in_state M state t ∗
+        {{{v k x f' , RET v; table_in_state M state t ∗
                              ((⌜v = NONEV⌝ ∗ ⌜complete M seq⌝) ∨
                               (⌜v = SOMEV ((k, x), f')⌝ ∗
-                               ⌜as_key k = Some k'⌝ ∗
-                               ⌜permitted M (seq ++ [(k', x)])⌝ ∗           
-                               ⌜is_cascade f' (seq ++ [(k', x)]) state t⌝)) }}} ;
+                               ⌜permitted M (seq ++ [(k, x)])⌝ ∗           
+                               ⌜is_cascade M f' (seq ++ [(k, x)]) state t⌝)) }}} ;
 
     table_cascade_spec M state t:
       {{{table_in_state M state t}}}
         table_cascade t
-        {{{f, RET f; ⌜is_cascade f [] state t⌝ ∗ table_in_state M state t }}}
+        {{{f, RET f; ⌜is_cascade M f [] state t⌝ ∗ table_in_state M state t }}}
   }.
+
+Print Implicit table_create.
+
+Arguments table_create {_ _ _ _ _ _ _ _ _ _ _ _ _ _ _ _} _.
+Arguments table_insert {_ _ _ _ _ _ _ _ _ _ _ _ _ _ _ _} _.
+Arguments table_lookup {_ _ _ _ _ _ _ _ _ _ _ _ _ _ _ _} _.
+Arguments table_fold {_ _ _ _ _ _ _ _ _ _ _ _ _ _ _ _} _.
+Arguments table_cascade {_ _ _ _ _ _ _ _ _ _ _ _ _ _ _ _} _.
+Arguments table_state {_ _ _ _ _ _ _ _ _ _ _ _ _ _ _ _} _.
+Arguments table_in_state {_ _ _ _ _ _ _ _ _ _ _ _ _ _ _ _ _} _ _ _.
+Arguments is_cascade {_ _ _ _ _ _ _ _ _ _ _ _ _ _ _ _ _} _ _ _ _ _.
+Arguments table_create_spec {_ _ _ _ _ _ _ _ _ _ _ _ _ _ _ _} _ _ _.
+Arguments table_insert_spec {_ _ _ _ _ _ _ _ _ _ _ _ _ _ _ _ _} _ _ _ _ _ _ _.
+Arguments table_lookup_spec {_ _ _ _ _ _ _ _ _ _ _ _ _ _ _ _ _} _ _ _ _ _ _.
+Arguments table_fold_spec {_ _ _ _ _ _ _ _ _ _ _ _ _ _ _ _ _} _ _ _ _ _ _ _.
+Arguments is_cascade_spec {_ _ _ _ _ _ _ _ _ _ _ _ _ _ _ _ _} _ _ _ _ _ _.
+Arguments table_cascade_spec {_ _ _ _ _ _ _ _ _ _ _ _ _ _ _ _ _} _ _ _.
+
+Existing Instances is_cascade_proper table_in_state_proper.
