iterators/hashtable_model_test.v
@@ -1,0 +1,267 @@
+From stdpp Require Import gmap.
+From iris.program_logic Require Import hoare.
+From iris_programs.iterators Require Import hashtable_invariants.
+From iris.heap_lang Require Import proofmode.
+
+Section tests.
+  
+  Context Σ `{!heapG Σ}.
+  
+  Definition equalf : val := λ: "x" "y", "x" = "y".
+  Definition idf : val := λ: "x", "x".
+  Definition as_natkey v :=
+    match v with
+    | #(LitInt z) => if decide (0 ≤ z)%Z then Some (Z.to_nat z) else None
+    | _ => None
+    end.
+  
+  Lemma as_natkey_inj v n:
+    as_natkey v = Some n -> v = #n.
+  Proof.
+    destruct v as [|l| | |]; try discriminate. destruct l as [n'| | |] ; try discriminate.
+    simpl ; case_decide ; last discriminate. intro Heq. injection Heq.
+    intro. rewrite -(Z2Nat.id n') ; last done.  by do 3 f_equal.
+  Qed.
+  
+  Lemma equalf_spec k1 k2 v1 v2 :
+    as_natkey v1 = Some k1 ->
+    as_natkey v2 = Some k2 ->
+    (WP (equalf v1) v2 {{ u, ⌜u = #(bool_decide (k1 = k2))⌝ }})%I.
+  Proof.
+    intros H1 H2. do 2 wp_lam. wp_op ; intro ; iPureIntro.
+    - simplify_eq. by rewrite bool_decide_true.
+    - rewrite bool_decide_false ; first reflexivity.
+      apply as_natkey_inj in H1. apply as_natkey_inj in H2. simplify_eq. by intros <-.
+  Qed.
+  
+  Lemma idhash_spec k v :
+    as_natkey v = Some k ->
+    (WP idf v {{ u, ⌜u = #(id k)⌝ }})%I.
+  Proof.
+    intro. wp_lam. eauto using as_natkey_inj.
+  Qed.
+
+  Instance nat_hashable : Hashable Σ nat id :=
+    {| equal_spec := equalf_spec ; hash_spec := idhash_spec  |}.
+
+  Parameter (table : Table Σ nat id (gmap nat)).
+
+  Lemma insert_nat_spec M (state :table_state table) t (n : nat) x :
+    {{{ table_in_state M state t }}}
+      table_insert table t #n x
+      {{{ (state' : table_state table), RET #();
+          table_in_state (insert_val M n x) state' t}}}.
+  Proof.
+    rewrite (_:Lit n = LitV n) ; last reflexivity.
+    eapply table_insert_spec.
+    simpl. rewrite decide_True. by rewrite Nat2Z.id. lia.
+  Qed.
+  
+  Definition test_1 : expr :=
+    let: "t" := table_create table #10 in
+    table_insert table "t" #1 #1 ;;
+    table_insert table "t" #2 #2 ;;
+    let: "a" := ref #0 in      
+    table_fold table (λ: "k" "x" <>, "a" <- !"a" + "x") "t" #() ;;
+    !"a".
+
+  Definition int_table : gmap nat _ -> iProp Σ :=
+    table_inv (fun _ v => ∃ (j : Z), ⌜v = #j⌝)%I.
+    
+  Fixpoint int_val_sum (seq : list (val)) :=
+    match seq with
+    | [] => Some 0%Z
+    |  #(LitInt x) :: seq => z ← int_val_sum seq ; Some (z + x)%Z
+    | _ => None
+    end.
+
+  Instance int_val_sum_proper : Proper ((≡ₚ) ==> (=)) int_val_sum.
+  Proof.
+    induction 1 as[|x|x y l| ???? Heq1 ? Heq2]. reflexivity.
+    - destruct x as [|x| | |]; try reflexivity. destruct x as [n| | |] ; try reflexivity.
+      simpl. by f_equal.
+    - destruct x as [|x| | |]; cycle 1 ; [destruct x|..] ; (destruct y as [|y| | |] ; cycle 1 ; [destruct y|..]) ; try reflexivity.
+      simpl. destruct (int_val_sum l) ; last reflexivity. simpl. f_equal. lia.
+    - by rewrite Heq1.
+  Qed.
+    
+
+  Lemma int_val_sum_app seq seq':
+    int_val_sum (seq ++ seq') = x ← int_val_sum seq ; y ← int_val_sum seq' ; Some (x + y)%Z.
+  Proof.
+    induction seq as [|x seq IH]. simpl. rewrite /mbind /option_bind ; by destruct (int_val_sum seq').
+    destruct x as [|x | | |] ; try reflexivity. destruct x ; try reflexivity.
+    simpl. rewrite IH. destruct (int_val_sum seq) ; last reflexivity.
+    destruct (int_val_sum seq') ; [simpl; f_equal; lia | reflexivity].
+  Qed.
+
+  Lemma int_val_sum_complete M seq:
+    complete M seq -> int_val_sum (seq.*2) = int_val_sum ((all_elements M).*2).
+  Proof.
+    intros HCom. pose proof (complete_all_elements _ _ HCom) as [seq' [Hseq <-]].
+    f_equal.
+    rewrite (_:forall l1 l2, iff (l1 = l2) (Forall2 (=) (l2) (l1))).
+    apply Forall2_fmap, (Forall2_impl _ _ _ _ Hseq).
+    by intros [??] [??] [<- _]. intros l1.
+    induction l1 as [|?? IH]. split.
+    intros <-. done.
+    intros. symmetry. by eapply Forall2_nil_inv_r.
+    split. intros <-. decompose_Forall.
+    intros HF. inversion HF. simplify_eq. f_equal. by apply IH.
+  Qed.
+    
+  Definition test_1_inv M l (seq: list (val * val)) (_ : val) : iProp Σ :=
+    ( int_table M ∗
+      ∃ i, ⌜int_val_sum (seq.*2) = Some i⌝
+          ∗ l ↦ #i)%I.
+  
+  Lemma test_1_inner M l k x seq a:
+    permitted M (seq ++ [(k,x)]) ->
+    {{test_1_inv M l seq a}} (λ: "k" "x" <>, #l <- !#l + "x") k x a {{v, test_1_inv M l (seq ++ [(k,x)]) v }}.
+  Proof.
+    intros [M' HRem]. iIntros "!# [HiTab Hl]".
+    iDestruct "Hl" as (i) "[% Hl]".
+    iDestruct (table_inv_removal _ _ _ _ HRem with "HiTab") as "[Hseq HiTabM']".
+    rewrite big_sepL_app big_sepL_singleton.
+    iDestruct "Hseq" as "[Hseq Hkx]".
+    iDestruct "Hkx" as (k') "[% Hx]".
+    iDestruct "Hx" as (j) "%". iSimplifyEq.
+    do 3 wp_lam. wp_load. wp_op. wp_store.
+    iSplit.
+    - iApply table_inv_removal ; first exact HRem.
+      iSplit.
+      + iApply big_sepL_app. iSplit. iAssumption.
+        iApply big_sepL_singleton. iExists k'. eauto.
+      + iAssumption.
+    - iExists (i + j). iFrame. iPureIntro.
+      rewrite fmap_app int_val_sum_app. by rewrite (_:int_val_sum (seq.*2) = Some i).
+  Qed.
+
+   
+  Lemma test_1_spec :
+    WP test_1 {{v, ⌜v = #3⌝}}%I.
+  Proof.
+    assert (H10: (10 > 0)%nat) ; first lia.
+    unfold test_1. rewrite (_:10%Z = 10%nat) ; last lia.
+    wp_bind (table_create _ _). iApply wp_wand.
+    iApply (table_create_spec _ _ H10).
+    iIntros (t) "HTable".
+    iDestruct "HTable" as (state) "HTable".
+    wp_lam. wp_apply (insert_nat_spec _ _ _ 1 #1 with "HTable").
+    iIntros (state') "HTable".
+    wp_lam. wp_apply (insert_nat_spec _ _ _ 2 #2 with "HTable").
+    iIntros (state'') "HTable".
+    wp_lam. wp_alloc a. wp_lam.
+    wp_apply (table_fold_spec _ _ _ (LamV "k" (λ: "x" <>, #a <- ! #a + "x")) _ #() with "[-]").
+    - intros. by eapply (test_1_inner _ _ ).
+    - iFrame. iSplit ; last eauto. rewrite /int_table. do 2 rewrite -table_inv_insert.
+      do 2 ( iSplit ; last eauto). iApply (table_inv_empty (Key:=nat)).
+    - iIntros (v seq) "[% [HTable [_ HInv]]]".
+      assert (HCom:complete (insert_val (insert_val ∅ 1%nat #1) 2%nat #2) seq) by assumption.
+      iDestruct "HInv" as (n) "[% Ha]".
+      assert (HSum: int_val_sum (seq.*2) = Some n) ; first assumption.
+      wp_seq. wp_load. iPureIntro. f_equal.
+      rewrite (int_val_sum_complete _ _ HCom) in HSum. vm_compute in HSum.
+      injection HSum. by intros <-.
+  Qed.
+
+   Definition test_2 (t : val) : expr :=
+    table_fold table (λ: <> "x" "a", "x" + "a")%V t #0.
+  
+  Lemma test_2_spec M (state : table_state table) t :
+    {{{int_table M ∗ table_in_state M state t}}}
+      test_2 t
+      {{{x, RET #x ; ⌜int_val_sum ((all_elements M).*2) = Some x⌝ ∗
+                     int_table M ∗ table_in_state M state t}}}.
+  Proof.
+    iIntros (Φ) "[HiTab HTable] HΦ".
+    wp_apply (table_fold_spec _ _  (fun seq v => int_table M ∗ ∃ x, ⌜int_val_sum (seq.*2) = Some x⌝ ∗ ⌜v = #x⌝)%I with "[HTable HiTab]").
+    - intros k x seq a [? HRem].
+      iIntros "!# [HiTab HInv]".
+      iDestruct "HInv" as (x') "[% %]". iSimplifyEq.
+      iDestruct (table_inv_removal _ _ _ _ HRem with "HiTab") as "[Hseq HiTabM']".
+      rewrite big_sepL_app big_sepL_singleton.
+      iDestruct "Hseq" as "[Hseq Hkx]".
+      iDestruct "Hkx" as (k') "[% Hx]".
+      iDestruct "Hx" as (j) "%". iSimplifyEq.
+      do 3 wp_lam. wp_op. iSplit.
+      + iApply table_inv_removal. done.
+        iSplit. iApply big_sepL_app. iSplit.
+        iAssumption. iApply big_sepL_singleton. eauto.
+        iAssumption.
+      + iExists (j + x')%Z. iSplit ; iPureIntro.
+        rewrite fmap_app int_val_sum_app (_:int_val_sum (seq.*2) = Some x') /=; last assumption.
+        f_equal. lia. reflexivity.
+    - eauto.
+    - iIntros (v seq) "[% [HTable [HiTab HInv]]]".
+      iDestruct "HInv" as (x) "[% %]". iSimplifyEq. iApply "HΦ".
+      iSplit. by erewrite <-int_val_sum_complete. iFrame.
+  Qed.
+
+  
+  Definition test_3 : expr :=
+    let: "t" := table_create table #10 in
+    table_insert table "t" #1 #1 ;;
+    table_insert table "t" #2 #2 ;;
+    let: "a" := ref #0 in
+    (rec: "loop" "c" :=
+       match: "c" #() with
+         NONE     => !"a"
+       | SOME "p" => "a" <- !"a" + Snd (Fst "p") ;;
+                     "loop" (Snd "p")
+       end) (table_cascade table "t").
+
+  Lemma test_3_spec :
+    WP test_3 {{ v, ⌜v = #3⌝ }}%I.
+  Proof.
+    assert (H10: (10 > 0)%nat) ; first lia.
+    unfold test_3. rewrite (_:10%Z = 10%nat) ; last lia.
+    wp_bind (table_create _ _). iApply wp_wand.
+    iApply (table_create_spec _ _  H10).
+    iIntros (t) "HTable".
+    iDestruct "HTable" as (state) "HTable".
+    wp_lam. wp_apply (insert_nat_spec _ _ _ 1 #1 with "HTable").
+    iIntros (state') "HTable".
+    wp_lam. wp_apply (insert_nat_spec _ _ _ 2 #2 with "HTable").
+    iIntros (state'') "HTable".
+    wp_lam. wp_alloc a. wp_lam.
+    wp_apply (table_cascade_spec with "HTable").
+    set (M:=(insert_val (insert_val ∅ 1%nat #1) 2%nat #2)).
+    iIntros (c) "[% HTable]". assert (Hcas:is_cascade M c [] state'' t) ; first assumption.
+    assert (Hloop: forall x seq,
+               int_val_sum (seq.*2) = Some x ->
+               is_cascade M c seq state'' t ->
+               table_in_state  M state'' t -∗ a ↦ #x -∗
+               WP (rec: "loop" "c" := match: "c" #() with
+                                        NONE => ! #a
+                                      | SOME "p" => #a <- ! #a + Snd (Fst "p") ;;
+                                                    "loop" (Snd "p")
+                                      end) c
+               {{ v, ⌜exists x seq, complete M seq /\ int_val_sum (seq.*2) = Some x /\ v = #x⌝ }}).
+    { clear Hcas.
+      intros i seq Hi Hcas. clear H.
+      iLöb as "IH" forall (c i seq Hi Hcas).
+      iIntros "HTable Ha".
+      wp_rec. wp_apply (is_cascade_spec with "HTable") ; first exact Hcas.
+      iIntros (? k x c') "[HTable [[% %]|[% [% %]]]]".
+      - simplify_eq. wp_match. wp_load. iPureIntro. exists i, seq. auto.
+      - simplify_eq. simpl.
+        assert (permitted M (seq ++ [(k, x)])) as [M' HRem] ; first assumption.
+        iAssert (int_table M) as "HiTab".
+        { do 2 (iApply (table_inv_insert (Key:=nat)) ; iSplit ; last eauto).
+          iApply (table_inv_empty (Key:=nat)).
+        }
+        iDestruct (table_inv_removal _ _ _ _ HRem with "HiTab") as "[Hseq _]".
+        rewrite big_sepL_app big_sepL_singleton.
+        iDestruct "Hseq" as "[_ Hkx]". iDestruct "Hkx" as (?) "[_ Hx]".
+        iDestruct "Hx" as (j) "%". iSimplifyEq.
+        wp_match. wp_load. do 2 wp_proj. wp_op. wp_store. wp_proj.
+        iApply ("IH" $! _ (i + j)%Z (seq ++ [(k , #j)]) with "[] [] HTable Ha").
+        by rewrite fmap_app int_val_sum_app Hi /=. done.
+    }
+    iApply (wp_wand with "[-]"). by iApply (Hloop 0 [] with "HTable [-]").
+    iIntros (v) "%".
+    assert (∃ (x : Z) (seq : list (val * val)), complete M seq ∧ int_val_sum (seq.*2) = Some x ∧ v = #x) as [x [seq [Hcom [Hsum ->]]]] ; first assumption.
+    rewrite (int_val_sum_complete _ _ Hcom) in Hsum.
+    vm_compute in Hsum. injection Hsum as <-. done.
+  Qed.
